Examples.v
@@ -1,4 +1,4 @@
-Require Import Process Eqdep_dec.
+Require Import Process Refinement.
 
 
 Module OnlyPositive.
@@ -19,46 +19,9 @@ Module OnlyPositive.
      end)
     || (#?chs["intermediate", n], #!chs["output", n], Done).
 
-  Theorem pr1_pr2 : refines (fun s => s = "input" \/ s = "output") pr1 pr2.
+  Theorem pr1_pr2 : refines pr1 pr2.
   Proof.
-    hnf; intros.
-    inversion H; clear H; subst; eauto.
-    apply (inj_pair2_eq_dec _ string_dec) in H2; subst.
-    destruct v.
-    inversion H3; clear H3; subst.
-    eexists; split.
-    econstructor.
-    econstructor.
-    instantiate (2 := O); simpl.
-    eauto.
-    eauto.
-    eauto.
-    eauto 10.
-
-    inversion H3; clear H3; subst.
-    Focus 2.
-    eexists; split.
-    econstructor.
-    repeat econstructor.
-    apply TrDone.
-    eauto.
-    eauto 10.
-
-    apply (inj_pair2_eq_dec _ string_dec) in H1; subst.
-    inversion H4; clear H4; subst.
-    eexists; split.
-    econstructor.
-    econstructor.
-    instantiate (2 := S v); simpl.
-    econstructor.
-    eauto.
-    econstructor.
-    econstructor.
-    econstructor.
-    apply IntCons1.
-    apply IntMatch1.
-    eauto.
-    eapply TrSome; eauto.
-    eapply TrSome; eauto.
+    refines.
+    destruct v; refines.
   Qed.
 End OnlyPositive.
