Refinement.v
@@ -1,0 +1,85 @@
+Require Import Process Eqdep_dec.
+
+
+Ltac inv H := inversion H; clear H; subst;
+              repeat match goal with
+                     | [ H : existT _ _ _ = existT _ _ _ |- _ ] =>
+                       apply (inj_pair2_eq_dec _ string_dec) in H; subst
+                     end.
+
+Section Refinement.
+  Variable chs : channels.
+
+  Theorem refines_refl : forall k,
+    refines (chs := chs) k k.
+  Proof.
+    intros; hnf; eauto.
+  Qed.
+
+  Theorem done_left : forall k,
+    refines (chs := chs) Done k.
+  Proof.
+    intros; hnf; intros.
+    inv H; eauto.
+  Qed.
+
+  Theorem done_right : forall k k',
+    refines k k'
+    -> refines (chs := chs) k (Done || k').
+  Proof.
+    intros; hnf; intros.
+    apply H in H0; firstorder.
+    eexists; split.
+    econstructor.
+    eauto.
+    eauto.
+    eauto.
+    auto.
+  Qed.
+
+  Theorem recv_recv : forall ch k k' k'',
+    (forall v, refines (k v) (k' v || k''))
+    -> refines (DoRecv (chs := chs) ch k) (DoRecv ch k' || k'').
+  Proof.
+    intros; hnf; intros.
+    inv H0; eauto.
+
+    apply H in H4; firstorder.
+    eexists; split.
+    inv H0.
+    econstructor.
+    econstructor.
+    eauto.
+    eauto.
+    econstructor; eauto.
+    econstructor.
+    econstructor.
+    econstructor.
+    econstructor.
+    eauto.
+    eauto.
+  Qed.
+
+  Theorem match_right : forall ch k k' k'' v,
+    refines k (k' || k'' v)
+    -> refines (chs := chs) k (DoSend ch v k' || DoRecv ch k'').
+  Proof.
+    intros; hnf; intros.
+    apply H in H0; firstorder.
+    inv H0; subst.
+    Focus 2.
+    inv H1; eauto.
+
+    eexists; split.
+    econstructor.
+    econstructor.
+    eauto.
+    econstructor.
+    eauto.
+    eauto.
+    auto.
+  Qed.
+End Refinement.
+
+Ltac refines := repeat (apply refines_refl || apply done_left || apply done_right
+                              || apply recv_recv || apply match_right; intros).
